

MARKSCHEME

1. prove that $1 + 2\left(\frac{1}{2}\right) + 3\left(\frac{1}{2}\right)^2 + 4\left(\frac{1}{2}\right)^3 + \dots + n\left(\frac{1}{2}\right)^{n-1} = 4 - \frac{n+2}{2^{n-1}}$
for $n = 1$
LHS = 1, RHS = $4 - \frac{1+2}{2^0} = 4 - 3 = 1$
so true for $n = 1$ R1
assume true for $n = k$ M1
so $1 + 2\left(\frac{1}{2}\right) + 3\left(\frac{1}{2}\right)^2 + 4\left(\frac{1}{2}\right)^3 + \dots + k\left(\frac{1}{2}\right)^{k-1} = 4 - \frac{k+2}{2^{k-1}}$
now for $n = k + 1$
LHS: $1 + 2\left(\frac{1}{2}\right) + 3\left(\frac{1}{2}\right)^2 + 4\left(\frac{1}{2}\right)^3 + \dots + k\left(\frac{1}{2}\right)^{k-1} + (k+1)\left(\frac{1}{2}\right)^k$ A1
 $= 4 - \frac{k+2}{2^{k-1}} + (k+1)\left(\frac{1}{2}\right)^k$ M1A1
 $= 4 - \frac{2(k+2)}{2^k} + \frac{k+1}{2^k}$ (or equivalent) A1
 $= 4 - \frac{(k+1)+2}{2^{(k+1)-1}}$ (accept $4 - \frac{k+3}{2^k}$) A1
Therefore if it is true for $n = k$ it is true for $n = k + 1$. It has been shown to be true for $n = 1$ so it is true for all $n \in \mathbb{Z}^+$. R1
Note: To obtain the final R mark, a reasonable attempt at induction must have been made.
- [8]
2. let $n = 1$
LHS = $1 \times 1! = 1$
RHS = $(1 + 1)! - 1 = 2 - 1 = 1$
hence true for $n = 1$ R1
assume true for $n = k$
$$\sum_{r=1}^k r(r!) = (k+1)! - 1$$
 M1
$$\sum_{r=1}^{k+1} r(r!) = (k+1)! - 1 + (k+1) \times (k+1)!$$
 M1A1
 $= (k+1)!(1 + k + 1) - 1$
 $= (k+1)!(k+2) - 1$ A1
 $= (k+2)! - 1$ A1
hence if true for $n = k$, true for $n = k + 1$ R1
since the result is true for $n = 1$ and $P(k) \Rightarrow P(k+1)$ the result is proved
by mathematical induction $\forall n \in \mathbb{Z}^+$ R1
- [8]
3. (a) (i) $1 \times 2 + 2 \times 3 + \dots + n(n+1) = \frac{1}{3}n(n+1)(n+2)$ R1
(ii) LHS = 40; RHS = 40 A1
(b) the sequence of values are:
5, 7, 11, 19, 35 ... or an example A1

35 is not prime, so Bill's conjecture is false

R1AG

(c) $P(n) : 5 \times 7^n + 1$ is divisible by 6

$P(1)$: 36 is divisible by 6 $\Rightarrow P(1)$ true

A1

assume $P(k)$ is true ($5 \times 7^k + 1 = 6r$)

M1

Note: Do **not** award M1 for statement starting 'let $n = k$ '.

Subsequent marks are independent of this M1.

consider $5 \times 7^{k+1} + 1$

M1

$= 7(6r - 1) + 1$

(A1)

$= 6(7r - 1) \Rightarrow P(k + 1)$ is true

A1

$P(1)$ true and $P(k)$ true $\Rightarrow P(k + 1)$ true, so by MI $P(n)$ is true for all $n \in \mathbb{Z}^+$ R1

Note: Only award R1 if there is consideration of $P(1)$, $P(k)$ and $P(k + 1)$ in the final statement.

Only award R1 if at least one of the two preceding A marks has been awarded.

[10]

4. (a) $S_6 = 81 \Rightarrow 81 = \frac{6}{2}(2a + 5d)$

M1A1

$\Rightarrow 27 = 2a + 5d$

$S_{11} = 231 \Rightarrow 231 = \frac{11}{2}(2a + 10d)$

M1A1

$\Rightarrow 21 = a + 5d$

solving simultaneously, $a = 6, d = 3$

A1A1

(b) $a + ar = 1$

A1

$a + ar + ar^2 + ar^3 = 5$

A1

$\Rightarrow (a + ar) + ar^2(1 + r) = 5$

$\Rightarrow 1 + ar^2 \times \frac{1}{a} = 5$

obtaining $r^2 - 4 = 0$

M1

$\Rightarrow r = \pm 2$

$r = 2$ (since all terms are positive)

A1

$a = \frac{1}{3}$

A1

(c) AP r^{th} term is $3r + 3$

A1

GP r^{th} term is $\frac{1}{3}2^{r-1}$

A1

$3(r + 1) \times \frac{1}{3}2^{r-1} = (r + 1)2^{r-1}$

M1AG

(d) prove: $P_n : \sum_{r=1}^n (r + 1)2^{r-1} = n2^n, n \in \mathbb{Z}^+$

show true for $n = 1$, i.e.

LHS $= 2 \times 2^0 = 2 = \text{RHS}$

A1

assume true for $n = k$, i.e.

M1

$\sum_{r=1}^k (r + 1)2^{r-1} = k2^k, k \in \mathbb{Z}^+$

consider $n = k + 1$

$\sum_{r=1}^{k+1} (r+1)2^{r-1} = k2^k + (k+1)2^k$	M1A1
$= 2^k(k + k + 2)$	
$= 2(k + 1)2^k$	A1
$= (k + 1)2^{k+1}$	A1
hence true for $n = k + 1$	
P_{k+1} is true whenever P_k is true, and P_1 is true, therefore P_n is true	R1
for $n \in \mathbb{Z}^+$	

[21]